coin.v
@@ -1,0 +1,239 @@
+From iris.program_logic Require Export weakestpre lifting.
+From iris.proofmode Require Import tactics.
+From iris_io Require Import lang rules.
+Require Import Coq.Logic.FunctionalExtensionality.
+
+
+CoFixpoint str_boolV (s : Stream bool) :=
+  {| Shead := BoolV (Shead s); Stail := str_boolV (Stail s) |}.
+
+CoFixpoint str_bool (s : Stream bool) :=
+  {| Shead := Bool (Shead s); Stail := str_bool (Stail s) |}.
+
+Lemma str_bool_vals (x : Stream bool) :
+  ∃ s : Stream val, proph_to_expr s = str_bool x.
+Proof.
+  exists (str_boolV x).
+  apply Seq_eq.
+  revert x. cofix IH => x.
+  rewrite [str_bool _]Stream_unfold; rewrite [proph_to_expr _]Stream_unfold.
+  destruct x; simpl.
+  econstructor; auto.
+Qed.
+
+Lemma str_bool_ent (n : nat) (s s' : Stream val) :
+    Elem (proph_to_expr s) str_bool →
+    Elem (proph_to_expr s') str_bool →
+    Elem (proph_to_expr (take_nth_from n s s')) str_bool.
+Proof.
+  intros [x Hx] [y Hy].
+  exists (take_nth_from n x y).
+  revert s s' x y Hx Hy; induction n => s s' x y.
+  - destruct x as [xh xt]; destruct y as [yh yt];
+      destruct s as [sh st]; destruct s' as [s'h s't]; simpl in *.
+    rewrite [str_bool _]Stream_unfold [proph_to_expr _]Stream_unfold => Hx.
+    rewrite [str_bool _]Stream_unfold [proph_to_expr _]Stream_unfold => Hy.
+    rewrite [str_bool _]Stream_unfold [proph_to_expr _]Stream_unfold.
+    simpl in *.
+    by inversion Hx; inversion Hy; simplify_eq.
+  - destruct x as [xh xt]; destruct y as [yh yt];
+      destruct s as [sh st]; destruct s' as [s'h s't]; simpl in *.
+    rewrite [str_bool _]Stream_unfold [proph_to_expr _]Stream_unfold => Hx.
+    rewrite [str_bool _]Stream_unfold [proph_to_expr _]Stream_unfold => Hy.
+    rewrite [str_bool _]Stream_unfold [proph_to_expr _]Stream_unfold.
+    simpl in *.
+    inversion Hx; inversion Hy; simplify_eq.
+    f_equal; auto.
+Qed.
+
+Lemma after_nth_const n b :
+  Nat.iter n Stail (str_bool (Sconst b)) = Sconst (#♭ b).
+Proof.
+  induction n.
+  - simpl.
+    apply Seq_eq.
+    cofix IH.
+    rewrite [Sconst (#♭ _)]Stream_unfold [str_bool _]Stream_unfold; simpl.
+    econstructor; auto.
+  - by simpl; rewrite IHn.
+Qed.
+
+Lemma str_bool_inh : ∃ p : Stream val, Elem (proph_to_expr p) str_bool.
+Proof.
+  exists (Sconst (BoolV true)), (Sconst true).
+  etrans; first apply (after_nth_const 0 true).
+  apply Seq_eq.
+  cofix IH.
+  rewrite [Sconst _]Stream_unfold; rewrite [proph_to_expr _]Stream_unfold; simpl.
+  econstructor; auto.
+Qed.
+
+Definition proph_after_nth_toss p n :=
+  PrP_eq (PrA p) (PrP p) (Stream bool) (λ x, Nat.iter n Stail (str_bool x)).
+
+Definition can_toss p b :=
+  ∃ z s, (PrP p z = s) ∧ (Shead s = (Bool b)).
+
+Lemma can_toss_after_nth p n b :
+  proph_after_nth_toss p n → can_toss p b.
+Proof.
+  intros [Heq1 Heq2].
+  destruct p as [pS pA pP pPv pPe pPSI]; simpl in *.
+  subst.
+  exists (Sconst b). exists (Sconst (Bool b)); simpl; split; auto.
+  rewrite Heq2.  apply after_nth_const.
+Qed.
+
+Lemma head_after_nth_toos p n :
+  proph_after_nth_toss p n → ∃ b, Shead (PrS p) = BoolV b.
+Proof.
+  intros [Heq1 Heq2].
+  destruct p as [pS pA pP pPv pPe pPSI]; simpl in *.
+  subst.
+  destruct pPSI as [x Hx].
+  destruct (pPv x) as [u Hu].
+  exists (Shead (Nat.iter n Stail x)).
+  rewrite Heq2 in Hx.
+  clear -Hx.
+  revert pS x Hx.
+  induction n => pS x Hx; simpl in *.
+  - destruct pS as [h t]; simpl in *.
+    apply (f_equal Shead) in Hx; simpl in *.
+    apply (f_equal to_val) in Hx; simpl in *.
+    by rewrite to_of_val in Hx; simplify_eq.
+  - rewrite -Nat_iter_S Nat_iter_S_r in Hx.
+    destruct x as [xh xt]; simpl in *.
+    apply IHn in Hx. rewrite Hx.
+    by rewrite -Nat_iter_S Nat_iter_S_r.
+Qed.
+
+Lemma proph_after_Snth_toss_tail p n :
+  proph_after_nth_toss p n →
+  proph_after_nth_toss (Proph_tail p) (S n).
+Proof.
+  intros [Heq1 Heq2].
+  destruct p as [pS pA pP pPv pPe pPSI]; simpl in *.
+  subst.
+  unshelve econstructor; eauto; simpl.
+  extensionality z.
+  by rewrite Heq2.
+Qed.
+
+Section coin.
+  Context `{heapIG Σ}.
+
+  Definition make_coin :=
+    Rec (Pair (Alloc (InjR Plang.Unit)) (Create_Pr _ str_bool)).
+
+  Definition flip :=
+    Rec (Rec ((Store (Var 3) (InjR Plang.Unit)))).
+
+  Definition read :=
+    Rec
+      (Rec
+         (Case
+            (Load (Var 3))
+            (Var 0)
+            (App
+               (Rec
+                  (App
+                     (Rec (App (Rec (Var 5)) (Assign_Pr (Var 6) (Var 3))))
+                     (Store (Var 6) (InjL (Var 1))))
+               )
+               Rand))).
+
+  Definition Coin (b : bool) (c l : loc) : iProp Σ :=
+    (∃ p, l ↦ₚ p ∗ ⌜ ∃ n, proph_after_nth_toss p n ⌝ ∗
+            (c ↦ (InjLV (BoolV b)) ∨ (c ↦ (InjRV UnitV)) ∗ ⌜Shead (PrS p) = BoolV b⌝))%I.
+
+  Lemma wp_make_coin :
+    {{{ True }}}
+      App make_coin Plang.Unit
+    {{{c l, RET PairV (LocV c) (PrV l); ∃ b, Coin b c l }}}.
+  Proof.
+    iIntros (Φ) "_ HΦ".
+    iApply wp_pure_step_later; auto; iNext.
+    asimpl.
+    iApply (wp_bind (fill [PairLCtx _])).
+    iApply wp_alloc; auto.
+    iNext. iIntros (c) "Hc"; simpl.
+    iApply (wp_bind (fill [PairRCtx (LocV _)])).
+    iApply wp_create_pr; auto using str_bool_vals, str_bool_ent, str_bool_inh.
+    iNext. iIntros (l) "Hl"; simpl. iDestruct "Hl" as (p) "[Hl Heq]".
+    iDestruct "Heq" as %Heq.
+    iApply wp_value. iApply "HΦ".
+    destruct (PrSI p) as [y Hy].
+    destruct (head_after_nth_toos p 0) as [b Hb]; auto.
+    iExists b.
+    iExists p; iFrame. iSplit; auto.
+    { iPureIntro. exists 0; simpl; auto. }
+  Qed.
+
+  Lemma wp_flip b c l :
+    {{{ Coin b c l }}} App (App flip (Loc c)) (Pr l) {{{RET UnitV; ∃ b, Coin b c l }}}.
+  Proof.
+    iIntros (Φ) "HC HΦ".
+    iApply (wp_bind (fill [AppLCtx _])).
+    iApply wp_pure_step_later; auto; iNext. asimpl.
+    iApply wp_value.
+    iApply wp_pure_step_later; auto; iNext. asimpl.
+    iDestruct "HC" as (p) "(Hl & HP & Hc)".
+    iDestruct "HP" as %[n HP].
+    pose proof (can_toss_after_nth _ n true HP).
+    iDestruct "Hc" as "[Hc|[Hc Hh]]".
+    - iApply (wp_store with "[$Hc]"). iNext. iIntros "Hc".
+      destruct (head_after_nth_toos p n) as [r Hr]; auto.
+      iApply "HΦ". iExists r.
+      iExists p; iFrame.
+      iSplit; eauto.
+    - iDestruct "Hh" as %Hh.
+      iApply (wp_store with "[$Hc]"). iNext. iIntros "Hc".
+      iApply "HΦ". iExists b.
+      iExists p; iFrame.
+      iSplit; eauto.
+  Qed.
+
+  Lemma wp_read b c l :
+    {{{ Coin b c l }}} App (App read (Loc c)) (Pr l) {{{RET (BoolV b); Coin b c l }}}.
+  Proof.
+    iIntros (Φ) "HC HΦ".
+    iApply (wp_bind (fill [AppLCtx _])).
+    iApply wp_pure_step_later; auto; iNext. asimpl.
+    iApply wp_value.
+    iApply wp_pure_step_later; auto; iNext. asimpl.
+    iDestruct "HC" as (p) "(Hl & HP & Hc)".
+    iDestruct "HP" as %[n HP].
+    iDestruct "Hc" as "[Hc|[Hc Hh]]".
+    - iApply (wp_bind (fill [CaseCtx _ _])).
+      iApply (wp_load with "[$Hc]"). iNext. iIntros "Hc". simpl.
+      iApply wp_pure_step_later; auto; iNext. asimpl.
+      iApply wp_value.
+      iApply "HΦ".
+      iExists p; iFrame.
+      iSplit; eauto.
+    - iDestruct "Hh" as %Hh.
+      iApply (wp_bind (fill [CaseCtx _ _])).
+      iApply (wp_load with "[$Hc]"). iNext. iIntros "Hc". simpl.
+      iApply wp_pure_step_later; auto; iNext. asimpl.
+      iApply (wp_bind (fill [AppRCtx (RecV _)])).
+      iApply wp_rand. iNext. iIntros (r) "!> /=".
+      iApply wp_pure_step_later; auto; iNext. asimpl.
+      iApply (wp_bind (fill [AppRCtx (RecV _)])).
+      iApply (wp_store with "[$Hc]"). iNext. iIntros "Hc". simpl.
+      iApply wp_pure_step_later; auto; iNext. asimpl.
+      iApply (wp_bind (fill [AppRCtx (RecV _)])).
+      iApply (wp_assign_pr with "[$Hl]").
+      { destruct (can_toss_after_nth p n r) as (z & s & Hz & Hs); eauto. }
+      iNext. iIntros "[HP Hl]". iDestruct "HP" as %HnP.
+      simpl.
+      iApply wp_pure_step_later; auto; iNext. asimpl.
+      iApply wp_value.
+      rewrite Hh in HnP. simplify_eq.
+      iApply "HΦ".
+      iExists _; iFrame.
+      iSplit; eauto.
+      iPureIntro.
+      exists (S n). by apply proph_after_Snth_toss_tail.
+  Qed.
+
+End coin.
